fix rsapss spec

specs/experimental/Spec.RSA.Bignum.fst
@@ -22,312 +22,290 @@ let bn_is_less x y = x < y
 
 type elem (n:bignum) = e:bignum{bn_v e < bn_v n}
 
-type sign =
-     | Positive : sign
-     | Negative : sign
-
-(* a - b = (sign, |a - b|) *)
-val abs_sub: 
-    x:size_nat -> a:bignum -> b:bignum -> Pure (tuple2 sign bignum)
-    (requires (a < pow2 (pow2 x) /\ b < pow2 (pow2 x)))
-    (ensures (fun (s, res) -> res < pow2 (pow2 x) /\ res = abs (a - b) /\
-			    s = (if a >= b then Positive else Negative)))
-    
-let abs_sub x a b =
-    if (bn_is_less a b)
-    then (Negative, b - a)
-    else (Positive, a - b)
-
-val add_sign:
-    c0:bignum -> c1:bignum -> c2:bignum ->
-    a0:bignum -> a1:bignum -> a2:bignum ->
-    b0:bignum -> b1:bignum -> b2:bignum ->
-    sa2:sign -> sb2:sign -> Pure bignum
-    (requires (c0 == a0 * b0 /\ c1 == a1 * b1 /\ c2 == a2 * b2 /\
-               a2 = abs (a0 - a1) /\ b2 = abs (b0 - b1) /\
-	       sa2 = (if (a0 >= a1) then Positive else Negative) /\
-	       sb2 = (if (b0 >= b1) then Positive else Negative)))
-    (ensures (fun res -> res == a1 * b0 + a0 * b1))
-
-#reset-options "--z3rlimit 150 --max_ifuel 0 --max_fuel 0"
-
-let add_sign c0 c1 c2 a0 a1 a2 b0 b1 b2 sa2 sb2 =
-    if ((sa2 = Positive && sb2 = Positive) || (sa2 = Negative && sb2 = Negative))
-    then (c0 + c1) - c2
-    else (c0 + c1) + c2
-
-val karatsuba:
-    x0:size_nat{0 < x0} -> a:bignum{a < pow2 (pow2 x0)} -> b:bignum{b < pow2 (pow2 x0)} -> Pure bignum
-    (requires (True))
-    (ensures (fun res -> res == a * b))
-    (decreases x0)
-
-#reset-options "--z3rlimit 300 --max_fuel 2"
-
-let rec karatsuba x0 a b =
-    if x0 < 9 then a * b
-    else begin
-        let x = x0 - 1 in
-        let pow_x = pow2 (pow2 x) in
-	
-        let a0 = a % pow_x in let a1 = a / pow_x in
-        assert (0 <= a0 /\ a0 < pow_x);
-        lemma_pow_div_karatsuba x0 a;
-        assert (0 <= a1 /\ a1 < pow_x);
-        lemma_div_mod a pow_x;
-
-        let b0 = b % pow_x in let b1 = b / pow_x in
-        assert (0 <= b0 /\ b0 < pow_x);
-        lemma_pow_div_karatsuba x0 b;
-        assert (0 <= b1 /\ b1 < pow_x);
-        lemma_div_mod b pow_x;
-
-        let (sa2, a2) = abs_sub x a0 a1 in
-        let (sb2, b2) = abs_sub x b0 b1 in
-		
-        let c0 = karatsuba x a0 b0 in
-        assert (c0 == a0 * b0); //from ind hypo
-        let c1 = karatsuba x a1 b1 in
-        assert (c1 == a1 * b1); //from ind hypo
-        let c2 = karatsuba x a2 b2 in
-        assert (c2 == a2 * b2); //from ind hypo
-		
-        let pow_x1 = pow2 (pow2 (x + 1)) in
-        let tmp = add_sign c0 c1 c2 a0 a1 a2 b0 b1 b2 sa2 sb2 in
-        let c = c1 * pow_x1 + tmp * pow_x + c0 in
-        lemma_karatsuba_mult x a a0 a1 b b0 b1;
-        assert (c == a * b);
-        c
-    end
-
-val get_ci: c:bignum -> i:size_nat -> Tot (res:bignum{res < pow2 64})
-let rec get_ci c i =
-    if (i = 0) then c % pow2 64
-    else get_ci (c / pow2 64) (i - 1)
-
 let beta = pow2 64
 
 val beta_i: i:size_nat -> Tot (res:bignum{res = pow2 (64 * i) /\ res > 0})
 let beta_i i = pow2 (64 * i)
 
-val lemma_beta_mul_by_beta_i: i:size_nat{i + 1 < max_size_t} -> Lemma
-    (requires (True))
-    (ensures (beta * beta_i i == beta_i (i + 1)))
-let lemma_beta_mul_by_beta_i i = admit()
-
-val lemma_mul_le: a:bignum -> b:bignum{b > 0} -> c:bignum{c > 0} -> Lemma
-    (requires (a <= b))
-    (ensures (a * c <= b * c))
-let lemma_mul_le a b c = ()
-
-val mont_reduction_:
-    n:bignum{n > 0} -> nInv_u64:bignum{nInv_u64 < beta} ->
-    exp_r:size_nat{0 < exp_r /\ exp_r + 1 < max_size_t} ->
-    c:bignum ->
-    i:size_nat{i <= exp_r} -> res:bignum -> Pure bignum
-    (requires (forall (j:size_nat). j <= i ==> res % n == c % n /\ res <= c + (beta_i i - 1) * n))
-    (ensures (fun res -> res % n == c % n /\ res <= c + (beta_i exp_r - 1) * n))
-    (decreases (exp_r - i))
-    #reset-options "--z3rlimit 150 --max_fuel 2"
-let rec mont_reduction_ n nInv_u64 exp_r c i res =
-    if (i < exp_r) then begin
-      let qi = (nInv_u64 * (get_ci res i)) % beta in
-      assert (0 <= qi /\ qi <= beta - 1);
-      let res1 = res + qi * (beta_i i) * n in
-      lemma_mod_plus res (qi * beta_i i) n; // res1 % n == res % n
-      assert (res1 <= c + (beta_i i - 1) * n + qi * beta_i i * n);
-      lemma_mul_le qi (beta - 1) (beta_i i * n);
-      assert (res1 <= c + (beta_i i - 1) * n + (beta - 1) * beta_i i * n);
-      assert (res1 <= c + beta_i i * n  - n + beta * beta_i i * n - beta_i i * n);
-      assert (res1 <= c - n + beta * beta_i i * n);
-      assert (res1 <= c + (beta * beta_i i - 1) * n);
-      lemma_beta_mul_by_beta_i i;
-      assert (res1 <= c + (beta_i (i + 1) - 1) * n);
-      mont_reduction_ n nInv_u64 exp_r c (i + 1) res1
-      end
-    else res
-     
-val mont_reduction:
-    n:bignum{n > 0} -> nInv_u64:bignum{nInv_u64 < beta} ->
-    exp_r:size_nat{0 < exp_r /\ exp_r + 1 < max_size_t} -> r:bignum{r == beta_i exp_r} ->
-    c:bignum{c < r * n} -> Pure (elem (n + n))
-    (requires (True))
-    (ensures (fun res -> res % n == (c / r) % n))
-    #reset-options "--z3rlimit 150 --max_fuel 0 --max_ifuel 0"
-let mont_reduction n nInv_u64 exp_r r c =
-    let tmp = mont_reduction_ n nInv_u64 exp_r c 0 c in
-    assert (tmp % n == c % n /\ tmp < c + (beta_i exp_r) * n);
-    let res = tmp / r in
-    assert (res % n = (tmp / r) % n);
-    lemma_mod_mult_div_1 tmp r n;
-    assert ((tmp / r) % n == ((c % n) / r) % n);
-    lemma_mod_mult_div_1 c r n;
-    assert (tmp < r * n + r * n);
-    assert (tmp < r * (n + n));
-    division_addition_lemma 0 r (n + n);
-    assert (res < n + n);
-    res
-
-val mul_mod_mont:
-    x0:size_nat ->
-    n:bignum{n > 0} -> nInv_u64:bignum{nInv_u64 < beta} ->
-    exp_r:size_nat{0 < exp_r /\ exp_r + 1 < max_size_t} -> r:bignum{r == beta_i exp_r /\ 4 * n < r} ->
-    a:elem (n + n) -> b:elem (n + n) -> Pure (elem (n + n))
-    (requires (True))
-    (ensures (fun res -> res % n == (a * b / r) % n))
-    #reset-options "--z3rlimit 50 --max_fuel 0"
-let mul_mod_mont x0 n nInv_u64 exp_r r a b =
-    //let c = karatsuba x0 a b in
-    let c = a * b in
-    assert (c < 4 * n * n);
-    mont_reduction n nInv_u64 exp_r r c
-
-val to_mont:
-    x0:size_nat ->
-    n:bignum{n > 0} -> nInv_u64:bignum{nInv_u64 < beta} ->
-    exp_r:size_nat{0 < exp_r /\ exp_r + 1 < max_size_t} -> r:bignum{r == beta_i exp_r /\ 4 * n < r} ->
-    r2:elem n -> a:elem n -> Pure (elem (n + n))
-    (requires (r2 == (r * r) % n))
-    (ensures (fun res -> res % n == (a * r) % n))
-    #reset-options "--z3rlimit 50 --max_fuel 0 --max_ifuel 0"
-let to_mont x0 n nInv_u64 exp_r r r2 a =
-    let c = a * r2 in
-    assert (c < n * n);
-    assert (c == a * ((r * r) % n));
-    let res = mont_reduction n nInv_u64 exp_r r c in
-    assert (res % n == ((a * ((r * r) % n)) / r) % n);
-    lemma_mod_div_simplify res a r n;
-    res
-
-val from_mont:
-    x0:size_nat ->
-    n:bignum{n > 0} -> nInv_u64:bignum{nInv_u64 < beta} ->
-    exp_r:size_nat{0 < exp_r /\ exp_r + 1 < max_size_t} -> r:bignum{r == beta_i exp_r /\ 4 * n < r} ->
-    a_r:elem (n + n) -> Pure (elem n)
-    (requires (True))
-    (ensures (fun res -> res == (a_r / r) % n))
-    #reset-options "--z3rlimit 50 --max_fuel 0 --max_ifuel 0"
-let from_mont x0 n nInv_u64 exp_r r a_r =
-    let tmp = mont_reduction_ n nInv_u64 exp_r a_r 0 a_r in
-    assert (tmp % n == a_r % n /\ tmp < a_r + (beta_i exp_r) * n);
-    let res = tmp / r in
-    assert (res % n = (tmp / r) % n);
-    lemma_mod_mult_div_1 tmp r n;
-    assert ((tmp / r) % n == ((a_r % n) / r) % n);
-    lemma_mod_mult_div_1 a_r r n;
-    assert (tmp < a_r + r * n);
-    lemma_div_le tmp (a_r + r * n) r;
-    assert (res <= (a_r + r * n) / r);
-    division_addition_lemma a_r r n;
-    assert (res <= a_r / r + n);
-    small_division_lemma_1 a_r r;
-    assert (res <= n); assume (res < n);
-    small_modulo_lemma_1 res n;
-    res
+val get_limbi: c:bignum -> i:size_nat -> Tot (res:bignum{res < pow2 64})
+let rec get_limbi c i =
+  if (i = 0) then c % pow2 64
+  else get_limbi (c / pow2 64) (i - 1)
 
 val mod_inv_u64_:
-    alpha:uint64 -> beta:uint64 ->
-    ub:uint64 -> vb:uint64 -> i:size_nat{i <= 64} -> Tot uint64
-    (decreases (64 - i))
+  alpha:uint64 -> beta:uint64 ->
+  ub:uint64 -> vb:uint64 -> i:size_nat{i <= 64} -> Tot uint64
+  (decreases (64 - i))
 let rec mod_inv_u64_ alpha beta ub vb i =
-    if (i < 64) then begin
-      let u_is_odd = u64 0 -. (ub &. u64 1) in
-      let beta_if_u_is_odd = beta &. u_is_odd in
-      let ub = ((ub ^. beta_if_u_is_odd) >>. (u32 1)) +. (ub &. beta_if_u_is_odd) in
+  if (i < 64) then begin
+    let u_is_odd = u64 0 -. (ub &. u64 1) in
+    let beta_if_u_is_odd = beta &. u_is_odd in
+    let ub = ((ub ^. beta_if_u_is_odd) >>. (u32 1)) +. (ub &. beta_if_u_is_odd) in
 
-      let alpha_if_u_is_odd = alpha &. u_is_odd in
-      let vb = (shift_right #U64 vb (u32 1)) +. alpha_if_u_is_odd in
-      mod_inv_u64_ alpha beta ub vb (i + 1) end 
-    else vb
+    let alpha_if_u_is_odd = alpha &. u_is_odd in
+    let vb = (shift_right #U64 vb (u32 1)) +. alpha_if_u_is_odd in
+    mod_inv_u64_ alpha beta ub vb (i + 1) end
+  else vb
 
 val mod_inv_u64: n0:uint64 -> Tot uint64
 let mod_inv_u64 n0 =
-    let alpha = shift_left #U64 (u64 1) (u32 63) in
-    let beta = n0 in
+  let alpha = shift_left #U64 (u64 1) (u32 63) in
+  let beta = n0 in
+  let ub = u64 1 in
+  let vb = u64 0 in
+  mod_inv_u64_ alpha beta ub vb 0
 
-    let ub = u64 1 in
-    let vb = u64 0 in
-    mod_inv_u64_ alpha beta ub vb 0
-  
+(* Karatsuba's multiplication *)
+type sign =
+  | Positive : sign
+  | Negative : sign
+
+// a - b = (sign, |a - b|)
+val abs_sub:
+  x:size_nat -> a:bignum -> b:bignum -> Pure (tuple2 sign bignum)
+  (requires (a < pow2 (pow2 x) /\ b < pow2 (pow2 x)))
+  (ensures (fun (s, res) -> res < pow2 (pow2 x) /\ res = abs (a - b) /\
+			  s = (if a >= b then Positive else Negative)))
+
+let abs_sub x a b =
+  if (bn_is_less a b)
+  then (Negative, b - a)
+  else (Positive, a - b)
+
+val add_sign:
+  c0:bignum -> c1:bignum -> c2:bignum ->
+  a0:bignum -> a1:bignum -> a2:bignum ->
+  b0:bignum -> b1:bignum -> b2:bignum ->
+  sa2:sign -> sb2:sign -> Pure bignum
+  (requires (c0 == a0 * b0 /\ c1 == a1 * b1 /\ c2 == a2 * b2 /\
+             a2 = abs (a0 - a1) /\ b2 = abs (b0 - b1) /\
+	     sa2 = (if (a0 >= a1) then Positive else Negative) /\
+	     sb2 = (if (b0 >= b1) then Positive else Negative)))
+  (ensures (fun res -> res == a1 * b0 + a0 * b1))
+
+let add_sign c0 c1 c2 a0 a1 a2 b0 b1 b2 sa2 sb2 =
+  if ((sa2 = Positive && sb2 = Positive) || (sa2 = Negative && sb2 = Negative))
+  then (c0 + c1) - c2
+  else (c0 + c1) + c2
+
+val karatsuba:
+  x0:size_nat ->
+  a:bignum{a < pow2 (pow2 x0)} -> b:bignum{b < pow2 (pow2 x0)} -> Tot (res:bignum{res == a * b})
+  (decreases x0)
+
+let rec karatsuba x0 a b =
+  if x0 < 9 then a * b
+  else begin
+    let x = x0 - 1 in
+    let pow_x = pow2 (pow2 x) in
+
+    let a0 = a % pow_x in let a1 = a / pow_x in
+    assert (0 <= a0 /\ a0 < pow_x);
+    lemma_pow_div_karatsuba x0 a;
+    assert (0 <= a1 /\ a1 < pow_x);
+    lemma_div_mod a pow_x;
+
+    let b0 = b % pow_x in let b1 = b / pow_x in
+    assert (0 <= b0 /\ b0 < pow_x);
+    lemma_pow_div_karatsuba x0 b;
+    assert (0 <= b1 /\ b1 < pow_x);
+    lemma_div_mod b pow_x;
+
+    let (sa2, a2) = abs_sub x a0 a1 in
+    let (sb2, b2) = abs_sub x b0 b1 in
+
+    let c0 = karatsuba x a0 b0 in
+    assert (c0 == a0 * b0); //from ind hypo
+    let c1 = karatsuba x a1 b1 in
+    assert (c1 == a1 * b1); //from ind hypo
+    let c2 = karatsuba x a2 b2 in
+    assert (c2 == a2 * b2); //from ind hypo
+
+    let pow_x1 = pow2 (pow2 (x + 1)) in
+    let tmp = add_sign c0 c1 c2 a0 a1 a2 b0 b1 b2 sa2 sb2 in
+    let c = c1 * pow_x1 + tmp * pow_x + c0 in
+    lemma_karatsuba_mult x a a0 a1 b b0 b1;
+    assert (c == a * b);
+    c
+  end
+
+(* Montgomery's arithmetic *)
+val mont_pred:
+  n:bignum{n > 0} -> exp_r:size_nat -> c:bignum -> i:size_nat{i <= exp_r} -> res:bignum -> Tot Type0
+let mont_pred n exp_r c i res = res % n = c % n && res <= c + (beta_i i - 1) * n
+
+val mont_reduction_f:
+  nInv_u64:bignum{nInv_u64 < beta} -> n:bignum{n > 0} ->
+  exp_r:size_nat{exp_r + 1 < max_size_t} -> c:bignum -> Tot (repeatable #bignum #exp_r (mont_pred n exp_r c))
+
+let mont_reduction_f nInv_u64 n exp_r c i res =
+  let qi = (nInv_u64 * (get_limbi res i)) % beta in
+  assert (0 <= qi /\ qi <= beta - 1);
+  let res1 = res + qi * (beta_i i) * n in
+  lemma_mod_plus res (qi * beta_i i) n; // res1 % n == res % n
+  assert (res1 <= c + (beta_i i - 1) * n + qi * beta_i i * n);
+  lemma_mul_le qi (beta - 1) (beta_i i * n);
+  assert (res1 <= c + (beta_i i - 1) * n + (beta - 1) * beta_i i * n);
+  assert (res1 <= c + beta_i i * n  - n + beta * beta_i i * n - beta_i i * n);
+  assert (res1 <= c - n + beta * beta_i i * n);
+  assert (res1 <= c + (beta * beta_i i - 1) * n);
+  lemma_beta_mul_by_beta_i i;
+  assert (res1 <= c + (beta_i (i + 1) - 1) * n);
+  res1
+
+val mont_reduction_:
+  nInv_u64:bignum{nInv_u64 < beta} -> n:bignum{n > 0} ->
+  exp_r:size_nat{exp_r + 1 < max_size_t} -> c:bignum -> Tot (res:bignum{res % n = c % n && res <= c + (beta_i exp_r - 1) * n})
+
+let mont_reduction_ nInv_u64 n exp_r c =
+  repeati_inductive exp_r (mont_pred n exp_r c) (mont_reduction_f nInv_u64 n exp_r c) c
+
+val mont_reduction:
+  nInv_u64:bignum{nInv_u64 < beta} -> n:bignum{n > 0} ->
+  exp_r:size_nat{exp_r + 1 < max_size_t} -> r:bignum{r == beta_i exp_r} ->
+  c:bignum{c < r * n} -> Tot (res:elem (n + n){res % n == (c / r) % n})
+  #reset-options "--z3rlimit 150 --max_fuel 0 --max_ifuel 0"
+let mont_reduction nInv_u64 n exp_r r c =
+  let tmp = mont_reduction_ nInv_u64 n exp_r c in
+  assert (tmp % n == c % n /\ tmp <= c + (beta_i exp_r - 1) * n);
+  assert (tmp < c + (beta_i exp_r) * n);
+  let res = tmp / r in
+  assert (res % n == (tmp / r) % n);
+  lemma_mod_mult_div_1 tmp r n;
+  assert (res % n == ((c % n) / r) % n);
+  lemma_mod_mult_div_1 c r n;
+  assert (res % n == (c / r) % n);
+
+  assert (tmp < r * n + r * n);
+  assert (tmp < r * (n + n));
+  lemma_div_exact_le tmp (n + n) r;
+  assert (res < n + n);
+  res
+
+val mul_mod_mont:
+  x0:size_nat ->
+  nInv_u64:bignum{nInv_u64 < beta} -> n:bignum{1 < n /\ 2 * n < pow2 (pow2 x0)} ->
+  exp_r:size_nat{exp_r + 1 < max_size_t} -> r:bignum{r == beta_i exp_r /\ 4 * n < r} ->
+  a:elem (n + n) -> b:elem (n + n) -> Tot (res:elem (n + n){res % n == (a * b / r) % n})
+  #reset-options "--z3rlimit 50 --max_fuel 0"
+let mul_mod_mont x0 nInv_u64 n exp_r r a b =
+  let c = karatsuba x0 a b in
+  //let c = a * b in
+  assert (c < 4 * n * n);
+  mont_reduction nInv_u64 n exp_r r c
+
+val to_mont:
+  x0:size_nat ->
+  nInv_u64:bignum{nInv_u64 < beta} -> n:bignum{1 < n /\ 2 * n < pow2 (pow2 x0)} ->
+  exp_r:size_nat{exp_r + 1 < max_size_t} -> r:bignum{r == beta_i exp_r /\ 4 * n < r} ->
+  r2:elem n -> a:elem n -> Pure (elem (n + n))
+  (requires (r2 == (r * r) % n))
+  (ensures (fun res -> res % n == (a * r) % n))
+  #reset-options "--z3rlimit 50 --max_fuel 0"
+let to_mont x0 nInv_u64 n exp_r r r2 a =
+  //let c = a * r2 in
+  let c = karatsuba x0 a r2 in
+  assert (c < n * n);
+  assert (c == a * ((r * r) % n));
+  let res = mont_reduction nInv_u64 n exp_r r c in
+  assert (res % n == ((a * ((r * r) % n)) / r) % n);
+  lemma_mod_div_simplify res a r n;
+  res
+
+val from_mont:
+  x0:size_nat ->
+  nInv_u64:bignum{nInv_u64 < beta} -> n:bignum{1 < n /\ 2 * n < pow2 (pow2 x0)} ->
+  exp_r:size_nat{exp_r + 1 < max_size_t} -> r:bignum{r == beta_i exp_r /\ 4 * n < r} ->
+  a_r:elem (n + n) -> Tot (res:elem n{res == (a_r / r) % n})
+
+let from_mont x0 nInv_u64 n exp_r r a_r =
+  let tmp = mont_reduction_ nInv_u64 n exp_r a_r in
+  assert (tmp % n == a_r % n /\ tmp <= a_r + (beta_i exp_r - 1) * n);
+  assert (tmp < a_r + (beta_i exp_r) * n);
+  let res = tmp / r in
+  assert (res % n = (tmp / r) % n);
+  lemma_mod_mult_div_1 tmp r n;
+  assert (res % n == ((a_r % n) / r) % n);
+  lemma_mod_mult_div_1 a_r r n;
+  assert (res % n == (a_r / r) % n);
+
+  (*assert (tmp < a_r + r * n);
+  lemma_div_le tmp (a_r + r * n) r;
+  assert (res <= (a_r + r * n) / r);
+  division_addition_lemma a_r r n;
+  assert (res <= a_r / r + n);
+  small_division_lemma_1 a_r r;
+  //assert (res <= n); *)
+  assume (res < n); //FIXME!!
+  small_modulo_lemma_1 res n;
+  assert (res == (a_r / r) % n);
+  res
+
 val mod_exp_:
-    x0:size_nat ->
-    n:bignum{n > 1} -> nInv_u64:bignum{nInv_u64 < beta} ->
-    exp_r:size_nat{0 < exp_r /\ exp_r + 1 < max_size_t} -> r:bignum{r == beta_i exp_r /\ 4 * n < r} ->
-    a:elem (n + n) -> b:bignum -> acc:elem (n + n) -> Pure (elem (n + n))
-    (requires True)
-    (ensures (fun res -> res % n == ((pow a b) * acc / pow r b) % n))
-    (decreases b)
-    #reset-options "--z3rlimit 150 --max_fuel 2"
-let rec mod_exp_ x0 n nInv_u64 exp_r r a b acc =
-    if b = 0
-    then acc
+  x0:size_nat ->
+  nInv_u64:bignum{nInv_u64 < beta} -> n:bignum{1 < n /\ 2 * n < pow2 (pow2 x0)} ->
+  exp_r:size_nat{exp_r + 1 < max_size_t} -> r:bignum{r == beta_i exp_r /\ 4 * n < r} ->
+  a:elem (n + n) -> b:bignum -> acc:elem (n + n) -> Tot (res:elem (n + n){res % n == ((pow a b) * acc / pow r b) % n})
+  (decreases b)
+  #reset-options "--z3rlimit 150 --max_fuel 2"
+let rec mod_exp_ x0 nInv_u64 n exp_r r a b acc =
+  if b = 0
+  then acc
+  else begin
+    let a2 = mul_mod_mont x0 nInv_u64 n exp_r r a a in
+    let b2 = bn_div2 b in
+    lemma_div_mod b 2;
+    if (bn_is_even b) then begin
+      assert (b = 2 * b2);
+      let res = mod_exp_ x0 nInv_u64 n exp_r r a2 b2 acc in
+      assert (res % n == ((pow a2 b2) * acc / pow r b2) % n); //from ind hypo
+      lemma_mod_exp n a a2 b b2 acc r res;
+      res end
     else begin
-        let a2 = mul_mod_mont x0 n nInv_u64 exp_r r a a in
-        let b2 = bn_div2 b in
-        lemma_div_mod b 2;
-        if (bn_is_even b) then begin
-            assert (b = 2 * b2);
-	    let res = mod_exp_ x0 n nInv_u64 exp_r r a2 b2 acc in
-            assert (res % n == ((pow a2 b2) * acc / pow r b2) % n); //from ind hypo
-            lemma_mod_exp n a a2 b b2 acc r res;
-            res end
-        else begin
-            assert (b = 2 * b2 + 1);
-            let acc' = mul_mod_mont x0 n nInv_u64 exp_r r a acc in
-            let res = mod_exp_ x0 n nInv_u64 exp_r r a2 b2 acc' in
-            assert (res % n == ((pow a2 b2) * acc' / pow r b2) % n); //from ind hypo
-            lemma_mod_exp_1 n a a2 b b2 acc acc' r res;
-            res end
-        end
+      assert (b = 2 * b2 + 1);
+      let acc' = mul_mod_mont x0 nInv_u64 n exp_r r a acc in
+      let res = mod_exp_ x0 nInv_u64 n exp_r r a2 b2 acc' in
+      assert (res % n == ((pow a2 b2) * acc' / pow r b2) % n); //from ind hypo
+      lemma_mod_exp_1 n a a2 b b2 acc acc' r res;
+      res end
+  end
 
 val mod_exp:
-    x0:size_nat -> modBits:size_nat{modBits > 0} ->
-    n:bignum{1 < n /\ n < pow2 modBits} -> a:elem n -> b:bignum -> Pure (elem n)
-    (requires True)
-    (ensures (fun res -> res == (pow a b) % n))
-    #reset-options "--z3rlimit 150 --max_fuel 0"
+  x0:size_nat -> modBits:size_nat{1 < modBits} ->
+  n:bignum{1 < n /\ n < pow2 modBits /\ 2 * n < pow2 (pow2 x0)} ->
+  a:elem n -> b:bignum -> Tot (res:elem n{res == (pow a b) % n})
+  #reset-options "--z3rlimit 50 --max_fuel 0"
 let mod_exp x0 modBits n a b =
-    let nLen = (modBits - 1) / 64 + 1 in
-    let exp_r = nLen + 1 in
-    let r = beta_i exp_r in
-    lemma_r_n modBits r n;
-    assert (4 * n < r);
-    let n0 = n % pow2 64 in
-    let n' = mod_inv_u64 (u64 n0) in
-    let nInv_u64 = uint_to_nat #U64 n' in
-    let r2 = (r * r) % n in
-    let a_r = to_mont x0 n nInv_u64 exp_r r r2 a in
-    let acc_r = to_mont x0 n nInv_u64 exp_r r r2 1 in
-    let res_r = mod_exp_ x0 n nInv_u64 exp_r r a_r b acc_r in
-    lemma_mod_exp_2 n a a_r b acc_r r res_r;
-    let res = from_mont x0 n nInv_u64 exp_r r res_r in
-    lemma_mod_mult_div_1 res_r r n;
-    lemma_mod_mult_div_1 ((pow a b) * r) r n;
-    multiple_division_lemma (pow a b) r;
-    res
+  let nLen = (modBits - 1) / 64 + 1 in
+  let exp_r = nLen + 1 in
+  let r = beta_i exp_r in
+  lemma_r_n modBits r n;
+  assert (4 * n < r);
+  let n0 = n % pow2 64 in
+  let nInv_u64 = uint_to_nat #U64 (mod_inv_u64 (u64 n0)) in
+  let r2 = (r * r) % n in
+  let a_r = to_mont x0 nInv_u64 n exp_r r r2 a in
+  let acc_r = to_mont x0 nInv_u64 n exp_r r r2 1 in
+  let res_r = mod_exp_ x0 nInv_u64 n exp_r r a_r b acc_r in
+  lemma_mod_exp_2 n a a_r b acc_r r res_r;
+  let res = from_mont x0 nInv_u64 n exp_r r res_r in
+  lemma_mod_mult_div_1 res_r r n;
+  lemma_mod_mult_div_1 ((pow a b) * r) r n;
+  multiple_division_lemma (pow a b) r;
+  res
 
 val rsa_blinding:
-    x0:size_nat ->
-    modBits:size_nat{1 < modBits /\ modBits + 3 < pow2 32} ->
-    n:bignum{1 < n /\ n < pow2 modBits /\ pow2 (modBits + 2) < pow2 (pow2 x0)} ->
-    p:elem n{1 < p} ->
-    q:elem n{1 < q /\ n = p * q} ->
-    d:elem n{1 < d} ->
-    m:elem n ->
-    rBlind:bignum{rBlind < pow2 64} -> Tot (s:bignum{s == (pow m d) % n})
+  x0:size_nat -> modBits:size_nat{1 < modBits} ->
+  n:bignum{1 < n /\ n < pow2 modBits /\ 2 * n < pow2 (pow2 x0)} ->
+  p:elem n{1 < p} -> q:elem n{1 < q /\ n = p * q} ->
+  d:elem n{1 < d} -> m:elem n ->
+  rBlind:bignum{rBlind < pow2 64} -> Tot (s:bignum{s == (pow m d) % n})
 
 let rsa_blinding x0 modBits n p q d m rBlind =
-    let phi_n:nat = (p - 1) * (q - 1) in
-    let d':nat = d + rBlind * phi_n in
-    let s = mod_exp x0 modBits n m d' in
-    assert (s == (pow m d') % n);
-    lemma_exp_blinding n phi_n p q d m rBlind;
-    assert (s == (pow m d) % n);
-    s
-
-(* BIGNUM CONVERT FUNCTIONS *)
-val os2ip:bLen:size_nat{bLen > 0} -> b:lbytes bLen -> Tot (res:bignum{res < pow2 (8 * bLen)})
-let os2ip bLen b = nat_from_intseq_be #U8 #bLen b
-
-val i2osp:n:bignum -> bLen:size_nat{n < pow2 (8 * bLen)} -> b:lbytes bLen -> Tot (lbytes bLen)
-let i2osp n bLen b = nat_to_bytes_be bLen n
+  let phi_n:nat = (p - 1) * (q - 1) in
+  let d':nat = d + rBlind * phi_n in
+  let s = mod_exp x0 modBits n m d' in
+  assert (s == (pow m d') % n);
+  lemma_exp_blinding n phi_n p q d m rBlind;
+  assert (s == (pow m d) % n);
+  s
