specs/experimental/Spec.RSA.Lemmas.fst
@@ -10,407 +10,395 @@ type elem (n:nat) = e:nat{e < n}
 #reset-options "--z3rlimit 30 --max_fuel 2"
 val pow : x:nat -> n:nat -> Tot nat
 let rec pow x n =
-    match n with
-    | 0 -> 1
-    | n -> x * pow x (n - 1)
+  match n with
+  | 0 -> 1
+  | n -> x * pow x (n - 1)
 
 val lemma_pow: x:nat -> n:nat -> m:nat -> Lemma
-    (pow x n * pow x m = pow x (n + m))
+  (pow x n * pow x m = pow x (n + m))
 let rec lemma_pow x n m =
-    let ass (x y z : nat) : Lemma ((x*y)*z == x*(y*z)) = () in
-    match n with
-    | 0 -> ()
-    | _ -> lemma_pow x (n-1) m; ass x (pow x (n-1)) (pow x m)
+  let ass (x y z : nat) : Lemma ((x*y)*z == x*(y*z)) = () in
+  match n with
+  | 0 -> ()
+  | _ -> lemma_pow x (n-1) m; ass x (pow x (n-1)) (pow x m)
 
 val lemma_pow_greater_0: a:nat{a > 0} -> b:nat -> Lemma
-    (requires True)
-    (ensures (pow a b > 0))
-    [SMTPat (pow a b)]
+  (pow a b > 0)
+  [SMTPat (pow a b)]
 let rec lemma_pow_greater_0 a b =
-    match b with
-    | 0 -> ()
-    | _ -> lemma_pow_greater_0 a (b - 1)
+  match b with
+  | 0 -> ()
+  | _ -> lemma_pow_greater_0 a (b - 1)
 
 val lemma_pow_0: b:nat{b > 0} -> Lemma (pow 0 b = 0)
 let rec lemma_pow_0 b =
-    match b with
-    | 1 -> ()
-    | _ -> lemma_pow_0 (b - 1)
+  match b with
+  | 1 -> ()
+  | _ -> lemma_pow_0 (b - 1)
 
 val lemma_pow_1: b:nat -> Lemma (pow 1 b = 1)
 let rec lemma_pow_1 b =
-    match b with
-    |  0 -> ()
-    | _ -> lemma_pow_1 (b - 1)
+  match b with
+  |  0 -> ()
+  | _ -> lemma_pow_1 (b - 1)
 
 #reset-options "--z3rlimit 30 --max_fuel 0"
 
 val lemma_pow_pow:
-    a:nat -> b:nat -> c:nat -> Lemma
-    (pow a (b * c) = pow (pow a b) c)
+  a:nat -> b:nat -> c:nat -> Lemma
+  (pow a (b * c) = pow (pow a b) c)
 let lemma_pow_pow a b c = admit()
 
 val lemma_pow_mul:
-    a:nat -> b:nat -> c:nat -> Lemma
-    (pow (a * b) c = (pow a c) * (pow b c))
+  a:nat -> b:nat -> c:nat -> Lemma
+  (pow (a * b) c = (pow a c) * (pow b c))
 let lemma_pow_mul a b c = admit()
 
 val lemma_pow_div:
-    a:nat -> b:nat -> d:nat{d > 0} -> Lemma
-    (pow (a / d) b = (pow a b) / pow d b)
+  a:nat -> b:nat -> d:nat{d > 0} -> Lemma
+  (pow (a / d) b = (pow a b) / pow d b)
 let lemma_pow_div a b d = admit()
 
 val lemma_pow_a2_b:
-    a:nat -> b:nat -> Lemma
-    (pow (a * a) b = pow a (2 * b))
+  a:nat -> b:nat -> Lemma
+  (pow (a * a) b = pow a (2 * b))
 let lemma_pow_a2_b a b =
-    lemma_pow_mul a a b;
-    lemma_pow a b b
+  lemma_pow_mul a a b;
+  lemma_pow a b b
 
 val lemma_pow_mod:
-    a:nat -> b:nat -> n:pos -> Lemma 
-    ((pow a b) % n == (pow (a % n) b) % n)
+  a:nat -> b:nat -> n:pos -> Lemma
+  ((pow a b) % n == (pow (a % n) b) % n)
 let lemma_pow_mod a b n = admit()
 
 val lemma_mod_mult_div_1:
-    a:nat -> d:nat{d > 0} -> n:nat{n > 0} -> Lemma
-    ((a / d) % n == ((a % n) / d) % n)
+  a:nat -> d:nat{d > 0} -> n:nat{n > 0} -> Lemma
+  ((a / d) % n == ((a % n) / d) % n)
 let lemma_mod_mult_div_1 a d n = admit()
 
 val lemma_mod_mult_div:
-    a:nat -> b:nat -> d:nat{d > 0} -> n:nat{n > 0} -> Lemma
-    ((a * b / d) % n == ((a % n) * b / d) % n)
+  a:nat -> b:nat -> d:nat{d > 0} -> n:nat{n > 0} -> Lemma
+  ((a * b / d) % n == ((a % n) * b / d) % n)
 let lemma_mod_mult_div a b d n =
-    lemma_mod_mult_div_1 (a * b) d n;
-    lemma_mod_mul_distr_l a b n;
-    lemma_mod_mult_div_1 ((a % n) * b) d n
+  lemma_mod_mult_div_1 (a * b) d n;
+  lemma_mod_mul_distr_l a b n;
+  lemma_mod_mult_div_1 ((a % n) * b) d n
 
 // (1 / d) % n is an inverse element of d
 val lemma_mult_div_mod:
-    a:nat -> b:nat -> d:nat{d > 0} -> n:nat{n > 0} -> Lemma
-    ((a * (b / d)) % n == (a * b / d) % n)
+  a:nat -> b:nat -> d:nat{d > 0} -> n:nat{n > 0} -> Lemma
+  ((a * (b / d)) % n == (a * b / d) % n)
 let lemma_mult_div_mod a b d n = admit()
- 
 
 (* LEMMAS for Montgomery's arithmetic *)
+val lemma_beta_mul_by_beta_i: i:size_nat{i + 1 < max_size_t} -> Lemma
+  (pow2 64 * pow2 (64 * i) == pow2 (64 * (i + 1)))
+let lemma_beta_mul_by_beta_i i =
+  pow2_plus 64 (64 * i)
 
-val lemma_mod_div_simplify: 
-    res:nat -> a:nat -> r:nat{r > 0} -> n:nat{n > 0} -> Lemma
-    (requires (res % n == (a * ((r * r) % n) / r) % n))
-    (ensures (res % n == (a * r) % n))
+val lemma_mul_le: a:nat -> b:nat{b > 0} -> c:nat{c > 0} -> Lemma
+  (requires (a <= b))
+  (ensures (a * c <= b * c))
+let lemma_mul_le a b c = ()
 
-#reset-options "--z3rlimit 50 --max_fuel 0"
+val lemma_div_exact_le:
+  a:nat -> b:nat -> c:nat{c > 0} -> Lemma
+  (requires (a < b * c))
+  (ensures (a / c < b))
+let lemma_div_exact_le a b c = ()
 
+val lemma_mod_div_simplify:
+  res:nat -> a:nat -> r:nat{r > 0} -> n:nat{n > 0} -> Lemma
+  (requires (res % n == (a * ((r * r) % n) / r) % n))
+  (ensures (res % n == (a * r) % n))
+  #reset-options "--z3rlimit 50 --max_fuel 0"
 let lemma_mod_div_simplify res a r n =
-    assert (res % n == (a * ((r * r) % n) / r) % n);
-    lemma_mod_mult_div (r * r) a r n;
-    paren_mul_right a r r;
-    paren_mul_left a r r;
-    multiple_division_lemma (a * r) r
+  assert (res % n == (a * ((r * r) % n) / r) % n);
+  lemma_mod_mult_div (r * r) a r n;
+  assert (res % n == (a * (r * r) / r) % n);
+  paren_mul_right a r r;
+  paren_mul_left a r r;
+  multiple_division_lemma (a * r) r
 
 (* LEMMAS for modular exponentiation *)
 
 val lemma_mult_abc:
-    a:nat -> b:nat -> c:nat -> Lemma
-    (a * b * c == a * c * b)
+  a:nat -> b:nat -> c:nat -> Lemma
+  (a * b * c == a * c * b)
 let lemma_mult_abc a b c = ()
 
 val lemma_r_n:
-    modBits:nat{modBits > 0} -> r:nat{r > 0} -> n:nat{n > 0} -> Lemma
-    (requires (r == pow2 (64 * ((modBits - 1) / 64 + 2)) /\ n < pow2 modBits))
-    (ensures (4 * n < r))
-    
+  modBits:nat{modBits > 0} -> r:nat{r > 0} -> n:nat{n > 0} -> Lemma
+  (requires (r == pow2 (64 * ((modBits - 1) / 64 + 2)) /\ n < pow2 modBits))
+  (ensures (4 * n < r))
 let lemma_r_n modBits r n =
-    assert (4 * n < 4 * pow2 modBits);
-    assert_norm (pow2 2 = 4);
-    pow2_plus 2 modBits;
-    assert (4 * n < pow2 (modBits + 2));
-    euclidean_division_definition (modBits - 1) 64;
-    assert (64 * ((modBits - 1) / 64) = modBits - 1 - (modBits - 1) % 64);
-    let exp2_r = 64 * ((modBits - 1) / 64 + 2) in
-    assert (exp2_r = 64 * ((modBits - 1) / 64) + 128);
-    assert (modBits + 63 < exp2_r);
-    pow2_lt_compat (modBits + 63) (modBits + 2);
-    pow2_lt_compat exp2_r (modBits + 63);
-    assert (4 * n < r)
+  assert (4 * n < 4 * pow2 modBits);
+  assert_norm (pow2 2 = 4);
+  pow2_plus 2 modBits;
+  assert (4 * n < pow2 (modBits + 2));
+  euclidean_division_definition (modBits - 1) 64;
+  assert (64 * ((modBits - 1) / 64) = modBits - 1 - (modBits - 1) % 64);
+  let exp2_r = 64 * ((modBits - 1) / 64 + 2) in
+  assert (exp2_r = 64 * ((modBits - 1) / 64) + 128);
+  assert (modBits + 63 < exp2_r);
+  pow2_lt_compat (modBits + 63) (modBits + 2);
+  pow2_lt_compat exp2_r (modBits + 63);
+  assert (4 * n < r)
 
 val lemma_mod_exp:
-    n:nat{n > 1} -> a:nat -> a2:nat ->
-    b:nat -> b2:nat -> acc:nat -> r:nat{r > 0} -> res:nat -> Lemma
-    (requires (a2 % n == (a * a / r) % n /\ b2 == b / 2 /\ 
-              res % n == ((pow a2 b2) * acc / pow r b2) % n))
-    (ensures (res % n == ((pow a (2 * b2)) * acc / pow r (2 * b2)) % n))
-    
+  n:nat{n > 1} -> a:nat -> a2:nat ->
+  b:nat -> b2:nat -> acc:nat -> r:nat{r > 0} -> res:nat -> Lemma
+  (requires (a2 % n == (a * a / r) % n /\ b2 == b / 2 /\
+             res % n == ((pow a2 b2) * acc / pow r b2) % n))
+  (ensures (res % n == ((pow a (2 * b2)) * acc / pow r (2 * b2)) % n))
 let lemma_mod_exp n a a2 b b2 acc r res =
-    lemma_mod_mult_div (pow a2 b2) acc (pow r b2) n;
-    lemma_pow_mod a2 b2 n;
-    lemma_pow_mod (a * a / r) b2 n;
-    lemma_pow_div (a * a) b2 r;
-    lemma_pow_a2_b a b2;
-    lemma_mod_mult_div (pow a (2 * b2) / pow r b2) acc (pow r b2) n;
-    lemma_mod_mult_div_1 ((pow a (2 * b2) / pow r b2) * acc) (pow r b2) n;
-    lemma_mult_div_mod acc (pow a (2 * b2)) (pow r b2) n;
-    lemma_mod_mult_div_1 ((acc * pow a (2 * b2)) / pow r b2) (pow r b2) n;
-    division_multiplication_lemma (acc * pow a (2 * b2)) (pow r b2) (pow r b2);
-    lemma_pow r b2 b2
+  lemma_mod_mult_div (pow a2 b2) acc (pow r b2) n;
+  lemma_pow_mod a2 b2 n;
+  lemma_pow_mod (a * a / r) b2 n;
+  lemma_pow_div (a * a) b2 r;
+  lemma_pow_a2_b a b2;
+  lemma_mod_mult_div (pow a (2 * b2) / pow r b2) acc (pow r b2) n;
+  lemma_mod_mult_div_1 ((pow a (2 * b2) / pow r b2) * acc) (pow r b2) n;
+  lemma_mult_div_mod acc (pow a (2 * b2)) (pow r b2) n;
+  lemma_mod_mult_div_1 ((acc * pow a (2 * b2)) / pow r b2) (pow r b2) n;
+  division_multiplication_lemma (acc * pow a (2 * b2)) (pow r b2) (pow r b2);
+  lemma_pow r b2 b2
 
 val lemma_mod_exp_1:
-    n:nat{n > 1} -> a:nat -> a2:nat ->
-    b:nat -> b2:nat -> acc:nat -> acc':nat -> r:nat{r > 0} -> res:nat -> Lemma
-    (requires (a2 % n == (a * a / r) % n /\ b2 == b / 2 /\ 
-               res % n == ((pow a2 b2) * acc' / pow r b2) % n /\
-               acc' % n == (a * acc / r) % n))
-    (ensures (res % n == ((pow a (2 * b2 + 1)) * acc / pow r (2 * b2 + 1)) % n))
-
-#reset-options "--z3rlimit 150 --max_fuel 0 --max_ifuel 0"
-
+  n:nat{n > 1} -> a:nat -> a2:nat ->
+  b:nat -> b2:nat -> acc:nat -> acc':nat -> r:nat{r > 0} -> res:nat -> Lemma
+  (requires (a2 % n == (a * a / r) % n /\ b2 == b / 2 /\
+             res % n == ((pow a2 b2) * acc' / pow r b2) % n /\
+             acc' % n == (a * acc / r) % n))
+  (ensures (res % n == ((pow a (2 * b2 + 1)) * acc / pow r (2 * b2 + 1)) % n))
 let lemma_mod_exp_1 n a a2 b b2 acc acc' r res =
-    assert (res % n == ((pow a2 b2) * acc' / pow r b2) % n);
-    lemma_mod_exp n a a2 b b2 acc' r res;
-    lemma_mod_mult_div acc' (pow a (2 * b2)) (pow r (2 * b2)) n;
-    lemma_mod_mult_div (a * acc / r) (pow a (2 * b2)) (pow r (2 * b2)) n;
-    lemma_mod_mult_div_1 ((pow a (2 * b2)) * (a * acc / r)) (pow r (2 * b2)) n;
-    lemma_mult_div_mod (pow a (2 * b2)) (a * acc) r n;
-    lemma_mod_mult_div_1 ((pow a (2 * b2)) * (a * acc) / r) ( pow r (2 * b2)) n;
-    division_multiplication_lemma ((pow a (2 * b2)) * (a * acc)) r (pow r (2 * b2));
-    paren_mul_right (pow a (2 * b2)) a acc;
-    paren_mul_left (pow a (2 * b2)) a acc;
-    assert_norm (pow a 1 = a);
-    lemma_pow a 1 (2 * b2);
-    assert_norm (pow r 1 = r);
-    lemma_pow r 1 (2 * b2)
+  assert (res % n == ((pow a2 b2) * acc' / pow r b2) % n);
+  lemma_mod_exp n a a2 b b2 acc' r res;
+  lemma_mod_mult_div acc' (pow a (2 * b2)) (pow r (2 * b2)) n;
+  lemma_mod_mult_div (a * acc / r) (pow a (2 * b2)) (pow r (2 * b2)) n;
+  lemma_mod_mult_div_1 ((pow a (2 * b2)) * (a * acc / r)) (pow r (2 * b2)) n;
+  lemma_mult_div_mod (pow a (2 * b2)) (a * acc) r n;
+  lemma_mod_mult_div_1 ((pow a (2 * b2)) * (a * acc) / r) ( pow r (2 * b2)) n;
+  division_multiplication_lemma ((pow a (2 * b2)) * (a * acc)) r (pow r (2 * b2));
+  paren_mul_right (pow a (2 * b2)) a acc;
+  paren_mul_left (pow a (2 * b2)) a acc;
+  assert_norm (pow a 1 = a);
+  lemma_pow a 1 (2 * b2);
+  assert_norm (pow r 1 = r);
+  lemma_pow r 1 (2 * b2)
 
 val lemma_mod_exp_2:
-    n:nat{n > 1} -> a:nat -> a_r:nat ->
-    b:nat -> acc_r:nat -> r:nat{r > 0} -> res_r:nat -> Lemma
-    (requires (a_r % n == (a * r) % n /\ acc_r % n == r % n /\
-               res_r % n == ((pow a_r b) * acc_r / pow r b) % n))
-    (ensures (res_r % n == ((pow a b) * r) % n))
-
-#reset-options "--z3rlimit 150 --max_fuel 0"
-
+  n:nat{n > 1} -> a:nat -> a_r:nat ->
+  b:nat -> acc_r:nat -> r:nat{r > 0} -> res_r:nat -> Lemma
+  (requires (a_r % n == (a * r) % n /\ acc_r % n == r % n /\
+             res_r % n == ((pow a_r b) * acc_r / pow r b) % n))
+  (ensures (res_r % n == ((pow a b) * r) % n))
+  #reset-options "--z3rlimit 50 --max_fuel 2"
 let lemma_mod_exp_2 n a a_r b acc_r r res_r =
-    assert (res_r % n == ((pow a_r b) * acc_r / pow r b) % n);
-    lemma_mod_mult_div (pow a_r b) acc_r (pow r b) n;
-    lemma_pow_mod a_r b n;
-    lemma_pow_mod (a * r) b n;
-    assert ((pow a_r b) % n == (pow (a * r) b) % n);
-    lemma_pow_mul a r b;
-    assert (res_r % n == (((pow a b * pow r b) % n) * acc_r / pow r b) % n);
-    lemma_mod_mult_div (pow a b * pow r b) acc_r (pow r b) n;
-    assert (res_r % n == (pow a b * (pow r b) * acc_r / pow r b) % n);
-    lemma_mult_abc (pow a b) (pow r b) acc_r;
-    multiple_division_lemma ((pow a b) * acc_r) (pow r b);
-    lemma_mod_mul_distr_l acc_r (pow a b) n;
-    lemma_mod_mul_distr_l r (pow a b) n
+  assert (res_r % n == ((pow a_r b) * acc_r / pow r b) % n);
+  lemma_mod_mult_div (pow a_r b) acc_r (pow r b) n;
+  lemma_pow_mod a_r b n;
+  lemma_pow_mod (a * r) b n;
+  assert ((pow a_r b) % n == (pow (a * r) b) % n);
+  lemma_pow_mul a r b;
+  assert (res_r % n == (((pow a b * pow r b) % n) * acc_r / pow r b) % n);
+  lemma_mod_mult_div (pow a b * pow r b) acc_r (pow r b) n;
+  assert (res_r % n == (pow a b * (pow r b) * acc_r / pow r b) % n);
+  lemma_mult_abc (pow a b) (pow r b) acc_r;
+  multiple_division_lemma ((pow a b) * acc_r) (pow r b);
+  lemma_mod_mul_distr_l acc_r (pow a b) n;
+  lemma_mod_mul_distr_l r (pow a b) n
 
 (* LEMMAS for exponent blinding *)
-
 val lemma_mod_pq:
-    a:nat -> b:nat -> p:nat{p > 1} -> q:nat{q > 1} -> Lemma
-    (requires (a % p == b % p /\ a % q == b % q))
-    (ensures (a % (p * q) == b % (p * q)))
+  a:nat -> b:nat -> p:nat{p > 1} -> q:nat{q > 1} -> Lemma
+  (requires (a % p == b % p /\ a % q == b % q))
+  (ensures (a % (p * q) == b % (p * q)))
 let lemma_mod_pq a b p q = admit()
 
 // m ^ (p - 1) = 1 (mod p) where gcd(m, p) = 1 and p is a prime number
 val fermat_little_theorem:
-    p:nat{p > 1} -> m:nat{m > 0} -> Lemma
-    (requires (m % p <> 0))
-    (ensures ((pow m (p - 1)) % p == 1))
+  p:nat{p > 1} -> m:nat{m > 0} -> Lemma
+  (requires (m % p <> 0))
+  (ensures ((pow m (p - 1)) % p == 1))
 let fermat_little_theorem p m = admit()
 
 val lemma_exp_blinding_q:
-    n:nat{n > 1} -> phi_n:nat -> p:elem n{p > 1} ->
-    q:elem n{q > 1} -> m:elem n{m > 0} -> Lemma
-    (requires (phi_n == (p - 1) * (q - 1) /\ n = p * q /\ m % q <> 0))
-    (ensures ((pow m phi_n) % q == 1))
-    
+  n:nat{n > 1} -> phi_n:nat -> p:elem n{p > 1} ->
+  q:elem n{q > 1} -> m:elem n{m > 0} -> Lemma
+  (requires (phi_n == (p - 1) * (q - 1) /\ n = p * q /\ m % q <> 0))
+  (ensures ((pow m phi_n) % q == 1))
+  #reset-options "--z3rlimit 50 --max_fuel 2"
 let lemma_exp_blinding_q n phi_n p q m =
-    let res = (pow m phi_n) % q in
-    lemma_pow_pow m (q - 1) (p - 1);
-    lemma_pow_mod (pow m (q - 1)) (p - 1) q;
-    fermat_little_theorem q m;
-    lemma_pow_1 (p - 1)
+  let res = (pow m phi_n) % q in
+  lemma_pow_pow m (q - 1) (p - 1);
+  lemma_pow_mod (pow m (q - 1)) (p - 1) q;
+  fermat_little_theorem q m;
+  lemma_pow_1 (p - 1)
 
 val lemma_exp_blinding_pq:
-    n:nat{n > 1} -> phi_n:nat -> p:elem n{p > 1} ->
-    q:elem n{q > 1} -> m:elem n{m > 0} -> Lemma
-    (requires (phi_n == (p - 1) * (q - 1) /\ n = p * q /\ m % p <> 0 /\ m % q <> 0))
-    (ensures ((pow m phi_n) % (p * q) == 1))
-    
+  n:nat{n > 1} -> phi_n:nat -> p:elem n{p > 1} ->
+  q:elem n{q > 1} -> m:elem n{m > 0} -> Lemma
+  (requires (phi_n == (p - 1) * (q - 1) /\ n = p * q /\ m % p <> 0 /\ m % q <> 0))
+  (ensures ((pow m phi_n) % (p * q) == 1))
+  #reset-options "--z3rlimit 50 --max_fuel 0"
 let lemma_exp_blinding_pq n phi_n p q m =
-    lemma_exp_blinding_q n phi_n p q m;
-    small_modulo_lemma_1 1 q;
-    lemma_exp_blinding_q n phi_n q p m;
-    small_modulo_lemma_1 1 p;
-    lemma_mod_pq (pow m phi_n) 1 p q;
-    small_modulo_lemma_1 1 n
+  lemma_exp_blinding_q n phi_n p q m;
+  small_modulo_lemma_1 1 q;
+  lemma_exp_blinding_q n phi_n q p m;
+  small_modulo_lemma_1 1 p;
+  lemma_mod_pq (pow m phi_n) 1 p q;
+  small_modulo_lemma_1 1 n
 
 val lemma_exp_blinding_1:
-    n:nat{n > 1} -> phi_n:nat -> p:elem n{p > 1} -> q:elem n{q > 1} ->
-    d:elem n{d > 0} -> m:elem n{m > 0} -> r:nat -> Lemma
-    (requires (phi_n = (p - 1) * (q - 1) /\ n = p * q /\ m % p <> 0 /\ m % q <> 0))
-    (ensures ((pow m (d + r * phi_n)) % n  == (pow m d) % n))
-
-#reset-options "--z3rlimit 150 --max_fuel 0"
-
+  n:nat{n > 1} -> phi_n:nat -> p:elem n{p > 1} -> q:elem n{q > 1} ->
+  d:elem n{d > 0} -> m:elem n{m > 0} -> r:nat -> Lemma
+  (requires (phi_n = (p - 1) * (q - 1) /\ n = p * q /\ m % p <> 0 /\ m % q <> 0))
+  (ensures ((pow m (d + r * phi_n)) % n  == (pow m d) % n))
 let lemma_exp_blinding_1 n phi_n p q d m r =
-    lemma_exp_blinding_pq n phi_n p q m;
-    assert ((pow m phi_n) % (p * q) == 1);
-    let res:nat = (pow m (d + r * phi_n)) % n in
-    lemma_pow m d (r * phi_n);
-    lemma_pow_pow m phi_n r;
-    lemma_pow_mod (pow m phi_n) r n;
-    assert ((pow (pow m phi_n) r) % n == (pow ((pow m phi_n) % n) r) % n);
-    assert ((pow (pow m phi_n) r) % n == (pow 1 r) % n);
-    lemma_pow_1 r;
-    modulo_lemma 1 n;
-    lemma_mod_mul_distr_l (pow m (r * phi_n)) (pow m d) n
+  lemma_exp_blinding_pq n phi_n p q m;
+  assert ((pow m phi_n) % (p * q) == 1);
+  let res:nat = (pow m (d + r * phi_n)) % n in
+  lemma_pow m d (r * phi_n);
+  lemma_pow_pow m phi_n r;
+  lemma_pow_mod (pow m phi_n) r n;
+  assert ((pow (pow m phi_n) r) % n == (pow ((pow m phi_n) % n) r) % n);
+  assert ((pow (pow m phi_n) r) % n == (pow 1 r) % n);
+  lemma_pow_1 r;
+  modulo_lemma 1 n;
+  lemma_mod_mul_distr_l (pow m (r * phi_n)) (pow m d) n
 
 val lemma_exp_blinding_0_q0:
-    n:nat{n > 1} -> phi_n:nat -> p:elem n{p > 1} -> q:elem n{q > 1} ->
-    d:elem n{d > 0} -> m:elem n{m > 0} -> r:nat -> Lemma
-    (requires (phi_n = (p - 1) * (q - 1) /\ n = p * q /\ m % q = 0))
-    (ensures ((pow m (d + r * phi_n)) % q == (pow m d) % q))
-    
+  n:nat{n > 1} -> phi_n:nat -> p:elem n{p > 1} -> q:elem n{q > 1} ->
+  d:elem n{d > 0} -> m:elem n{m > 0} -> r:nat -> Lemma
+  (requires (phi_n = (p - 1) * (q - 1) /\ n = p * q /\ m % q = 0))
+  (ensures ((pow m (d + r * phi_n)) % q == (pow m d) % q))
 let lemma_exp_blinding_0_q0 n phi_n p q d m r =
-    let res:nat = pow m (d + r * phi_n) in
-    assert (res % q == (pow m (d + r * phi_n)) % q);
-    lemma_pow_mod m (d + r * phi_n) q;
-    lemma_pow_0 (d + r * phi_n);
-    lemma_pow_mod m d q;
-    lemma_pow_0 d
+  let res:nat = pow m (d + r * phi_n) in
+  assert (res % q == (pow m (d + r * phi_n)) % q);
+  lemma_pow_mod m (d + r * phi_n) q;
+  lemma_pow_0 (d + r * phi_n);
+  lemma_pow_mod m d q;
+  lemma_pow_0 d
 
 val lemma_exp_blinding_0_q1:
-    n:nat{n > 1} -> phi_n:nat -> p:elem n{p > 1} -> q:elem n{q > 1} ->
-    d:elem n{d > 0} -> m:elem n{m > 0} -> r:nat -> Lemma
-    (requires (phi_n = (p - 1) * (q - 1) /\ n = p * q /\ m % p <> 0))
-    (ensures ((pow m (d + r * phi_n)) % p == (pow m d) % p))
-
-#reset-options "--z3rlimit 150 --max_fuel 0"
-
+  n:nat{n > 1} -> phi_n:nat -> p:elem n{p > 1} -> q:elem n{q > 1} ->
+  d:elem n{d > 0} -> m:elem n{m > 0} -> r:nat -> Lemma
+  (requires (phi_n = (p - 1) * (q - 1) /\ n = p * q /\ m % p <> 0))
+  (ensures ((pow m (d + r * phi_n)) % p == (pow m d) % p))
 let lemma_exp_blinding_0_q1 n phi_n p q d m r =
-    lemma_exp_blinding_q n phi_n q p m;
-    assert ((pow m phi_n) % p == 1);
-    let res:nat = pow m (d + r * phi_n) in
-    assert (res % p == (pow m (d + r * phi_n)) % p);
-    lemma_pow m d (r * phi_n);
-    assert (res % p == ((pow m d) * (pow m (r * phi_n))) % p);
-    lemma_mod_mul_distr_l (pow m (r * phi_n)) (pow m d) p;
-    lemma_pow_pow m phi_n r;
-    lemma_pow_mod (pow m phi_n) r p;
-    assert ((pow m (r * phi_n)) % p == (pow ((pow m phi_n) % p) r) % p);
-    assert ((pow (pow m phi_n) r) % p == (pow 1 r) % p);
-    lemma_pow_1 r;
-    modulo_lemma 1 p;
-    assert (res % p == ((pow m d) * 1) % p) 
+  lemma_exp_blinding_q n phi_n q p m;
+  assert ((pow m phi_n) % p == 1);
+  let res:nat = pow m (d + r * phi_n) in
+  assert (res % p == (pow m (d + r * phi_n)) % p);
+  lemma_pow m d (r * phi_n);
+  assert (res % p == ((pow m d) * (pow m (r * phi_n))) % p);
+  lemma_mod_mul_distr_l (pow m (r * phi_n)) (pow m d) p;
+  lemma_pow_pow m phi_n r;
+  lemma_pow_mod (pow m phi_n) r p;
+  assert ((pow m (r * phi_n)) % p == (pow ((pow m phi_n) % p) r) % p);
+  assert ((pow (pow m phi_n) r) % p == (pow 1 r) % p);
+  lemma_pow_1 r;
+  modulo_lemma 1 p;
+  assert (res % p == ((pow m d) * 1) % p)
 
 val lemma_exp_blinding_0_q:
-    n:nat{n > 1} -> phi_n:nat -> p:elem n{p > 1} -> q:elem n{q > 1} ->
-    d:elem n{d > 0} -> m:elem n{m > 0} -> r:nat -> Lemma
-    (requires (phi_n = (p - 1) * (q - 1) /\ n = p * q /\ m % q = 0 /\ m % p <> 0))
-    (ensures ((pow m (d + r * phi_n)) % n == (pow m d) % n))
-    
+  n:nat{n > 1} -> phi_n:nat -> p:elem n{p > 1} -> q:elem n{q > 1} ->
+  d:elem n{d > 0} -> m:elem n{m > 0} -> r:nat -> Lemma
+  (requires (phi_n = (p - 1) * (q - 1) /\ n = p * q /\ m % q = 0 /\ m % p <> 0))
+  (ensures ((pow m (d + r * phi_n)) % n == (pow m d) % n))
 let lemma_exp_blinding_0_q n phi_n p q d m r =
-    let res:nat = pow m (d + r * phi_n) in
-    lemma_exp_blinding_0_q0 n phi_n p q d m r;
-    lemma_exp_blinding_0_q1 n phi_n p q d m r;
-    lemma_mod_pq res (pow m d) p q;
-    assert (res % n == (pow m d) % n)
+  let res:nat = pow m (d + r * phi_n) in
+  lemma_exp_blinding_0_q0 n phi_n p q d m r;
+  lemma_exp_blinding_0_q1 n phi_n p q d m r;
+  lemma_mod_pq res (pow m d) p q;
+  assert (res % n == (pow m d) % n)
 
 val lemma_exp_blinding_0_pq:
-    n:nat{n > 1} -> phi_n:nat -> p:elem n{p > 1} -> q:elem n{q > 1} ->
-    d:elem n{d > 0} -> m:elem n -> r:nat -> Lemma
-    (requires (phi_n = (p - 1) * (q - 1) /\ n = p * q /\ m % q = 0 /\ m % p = 0))
-    (ensures ((pow m (d + r * phi_n)) % n == (pow m d) % n))
-    
+  n:nat{n > 1} -> phi_n:nat -> p:elem n{p > 1} -> q:elem n{q > 1} ->
+  d:elem n{d > 0} -> m:elem n -> r:nat -> Lemma
+  (requires (phi_n = (p - 1) * (q - 1) /\ n = p * q /\ m % q = 0 /\ m % p = 0))
+  (ensures ((pow m (d + r * phi_n)) % n == (pow m d) % n))
 let lemma_exp_blinding_0_pq n phi_n p q d m r =
-    small_modulo_lemma_1 0 p;
-    small_modulo_lemma_1 0 q;
-    lemma_mod_pq m 0 p q;
-    small_modulo_lemma_1 0 n;
-    assert (m % n == 0);
-    small_modulo_lemma_1 m n;
-    assert (m = 0);
-    lemma_pow_0 (d + r * phi_n);
-    lemma_pow_0 d
+  small_modulo_lemma_1 0 p;
+  small_modulo_lemma_1 0 q;
+  lemma_mod_pq m 0 p q;
+  small_modulo_lemma_1 0 n;
+  assert (m % n == 0);
+  small_modulo_lemma_1 m n;
+  assert (m = 0);
+  lemma_pow_0 (d + r * phi_n);
+  lemma_pow_0 d
 
 val lemma_exp_blinding_0:
-    n:nat{n > 1} -> phi_n:nat -> p:elem n{p > 1} -> q:elem n{q > 1} ->
-    d:elem n{d > 0} -> m:elem n -> r:nat -> Lemma
-    (requires (phi_n = (p - 1) * (q - 1) /\ n = p * q /\ 
-                (m = 0 \/ m % p = 0 \/ m % q = 0)))
-    (ensures ((pow m (d + r * phi_n)) % n  == (pow m d) % n))
-    
+  n:nat{n > 1} -> phi_n:nat -> p:elem n{p > 1} -> q:elem n{q > 1} ->
+  d:elem n{d > 0} -> m:elem n -> r:nat -> Lemma
+  (requires (phi_n = (p - 1) * (q - 1) /\ n = p * q /\
+            (m = 0 \/ m % p = 0 \/ m % q = 0)))
+  (ensures ((pow m (d + r * phi_n)) % n  == (pow m d) % n))
 let lemma_exp_blinding_0 n phi_n p q d m r =
-    if (m = 0) then begin
-        lemma_pow_0 (d + r * phi_n);
-        lemma_pow_0 d end
+  if (m = 0) then begin
+    lemma_pow_0 (d + r * phi_n);
+    lemma_pow_0 d end
+  else begin
+    if (m % p = 0 && m % q <> 0) then
+      lemma_exp_blinding_0_q n phi_n q p d m r
     else begin
-        if (m % p = 0 && m % q <> 0) then
-            lemma_exp_blinding_0_q n phi_n q p d m r
-        else begin
-            if (m % q = 0 && m % p <> 0) then
-                lemma_exp_blinding_0_q n phi_n p q d m r
-                else begin
-                    assert (m % p = 0 && m % q = 0);
-                    lemma_exp_blinding_0_pq n phi_n p q d m r end
-            end
-        end
+      if (m % q = 0 && m % p <> 0) then
+	lemma_exp_blinding_0_q n phi_n p q d m r
+      else begin
+	assert (m % p = 0 && m % q = 0);
+	lemma_exp_blinding_0_pq n phi_n p q d m r end
+    end
+  end
 
 val lemma_exp_blinding:
-    n:nat{n > 1} -> phi_n:nat -> p:elem n{p > 1} -> q:elem n{q > 1} ->
-    d:elem n{d > 0} -> m:elem n -> r:nat -> Lemma
-    (requires (phi_n = (p - 1) * (q - 1) /\ n = p * q))
-    (ensures ((pow m (d + r * phi_n)) % n  == (pow m d) % n))
-    
+  n:nat{n > 1} -> phi_n:nat -> p:elem n{p > 1} -> q:elem n{q > 1} ->
+  d:elem n{d > 0} -> m:elem n -> r:nat -> Lemma
+  (requires (phi_n = (p - 1) * (q - 1) /\ n = p * q))
+  (ensures ((pow m (d + r * phi_n)) % n  == (pow m d) % n))
 let lemma_exp_blinding n phi_n p q d m r =
-    if (m = 0 || m % p = 0 || m % q = 0) then 
-        lemma_exp_blinding_0 n phi_n p q d m r
-    else lemma_exp_blinding_1 n phi_n p q d m r
+  if (m = 0 || m % p = 0 || m % q = 0) then
+    lemma_exp_blinding_0 n phi_n p q d m r
+  else lemma_exp_blinding_1 n phi_n p q d m r
 
 (* LEMMAS for Karatsuba's multiplication *)
+val abs: x:int -> Tot (y:nat{(x >= 0 ==> y = x) /\ (x < 0 ==> y = -x)})
+let abs x = if x >= 0 then x else -x
 
-val lemma_distributivity_mult: 
-    a:nat -> b:nat -> c:nat -> d:nat -> Lemma
-    ((a + b) * (c + d) = a * c + a * d + b * c + b * d)
+val lemma_distributivity_mult:
+  a:nat -> b:nat -> c:nat -> d:nat -> Lemma
+  ((a + b) * (c + d) = a * c + a * d + b * c + b * d)
 let lemma_distributivity_mult a b c d = ()
 
 val lemma_karatsuba_mult:
-    x:size_nat -> a:nat -> a0:nat -> a1:nat -> b:nat -> b0:nat -> b1:nat -> Lemma
-    (requires (let pow_x = pow2 (pow2 x) in
-	      a == a1 * pow_x + a0 /\ b == b1 * pow_x + b0))
-    (ensures (let pow_x = pow2 (pow2 x) in
-	      let pow_x1 = pow2 (pow2 (x + 1)) in
-	      a * b == a1 * b1 * pow_x1 + (a0 * b1 + a1 * b0) * pow_x + a0 * b0))
-
-#reset-options "--z3rlimit 150 --initial_fuel 0 --max_fuel 0"
-
+  x:size_nat -> a:nat -> a0:nat -> a1:nat -> b:nat -> b0:nat -> b1:nat -> Lemma
+  (requires (let pow_x = pow2 (pow2 x) in
+	     a == a1 * pow_x + a0 /\ b == b1 * pow_x + b0))
+  (ensures (let pow_x = pow2 (pow2 x) in
+	    let pow_x1 = pow2 (pow2 (x + 1)) in
+	    a * b == a1 * b1 * pow_x1 + (a0 * b1 + a1 * b0) * pow_x + a0 * b0))
+  #reset-options "--z3rlimit 50 --max_fuel 2"
 let lemma_karatsuba_mult x a a0 a1 b b0 b1 =
-    let pow_x = pow2 (pow2 x) in
-    let pow_x1 = pow2 (pow2 (x + 1)) in
-    assert (a * b == (a1 * pow_x + a0) * (b1 * pow_x + b0));
-    lemma_distributivity_mult (a1 * pow_x) a0 (b1 * pow_x) b0;
-    pow2_plus (pow2 x) (pow2 x);
-    pow2_double_sum x
+  let pow_x = pow2 (pow2 x) in
+  let pow_x1 = pow2 (pow2 (x + 1)) in
+  assert (a * b == (a1 * pow_x + a0) * (b1 * pow_x + b0));
+  lemma_distributivity_mult (a1 * pow_x) a0 (b1 * pow_x) b0;
+  pow2_plus (pow2 x) (pow2 x);
+  pow2_double_sum x
 
 val lemma_pow_div_karatsuba:
-    x0:size_nat{x0 > 0} -> b:nat{b < pow2 (pow2 x0)} -> Lemma
-    (requires (True))
-    (ensures (let pow_x = pow2 (pow2 (x0 - 1)) in
-	      let b1 = b / pow_x in
-	      0 <= b1 /\ b1 < pow_x))
-
-#reset-options "--z3rlimit 100 --initial_fuel 0 --max_fuel 0"
-
+  x0:size_nat{x0 > 0} -> b:nat{b < pow2 (pow2 x0)} -> Lemma
+  (requires (True))
+  (ensures (let pow_x = pow2 (pow2 (x0 - 1)) in
+	    let b1 = b / pow_x in
+	    0 <= b1 /\ b1 < pow_x))
+  #reset-options "--z3rlimit 150 --max_fuel 0"
 let lemma_pow_div_karatsuba x0 b =
-    let x = x0 - 1 in
-    let pow_x = pow2 (pow2 x) in
-    pow2_lt_compat x0 x;
-    lemma_div_lt b (pow2 x0) (pow2 x);
-    assert (b / pow_x < pow2 (pow2 x0 - pow2 x));
-    pow2_plus (x0 - 1) 1;
-    assert_norm (pow2 1 = 2)
-
-val abs: x:int -> Tot (y:nat{(x >= 0 ==> y = x) /\ (x < 0 ==> y = -x)})
-let abs x = if x >= 0 then x else -x
+  let x = x0 - 1 in
+  let pow_x = pow2 (pow2 x) in
+  pow2_lt_compat x0 x;
+  lemma_div_lt b (pow2 x0) (pow2 x);
+  assert (b / pow_x < pow2 (pow2 x0 - pow2 x));
+  pow2_plus (x0 - 1) 1;
+  assert_norm (pow2 1 = 2)
