specs/experimental/Spec.RSA.fst
@@ -4,9 +4,8 @@ open FStar.Mul
 open Spec.Lib.IntTypes
 open Spec.Lib.IntSeq
 open Spec.Lib.RawIntTypes
-
 open FStar.Math.Lemmas
-open Spec.RSA.Lemmas
+
 open Spec.RSA.Bignum
 
 module Hash = Spec.SHA2
@@ -16,261 +15,211 @@ module Hash = Spec.SHA2
 val blocks: x:size_nat{x > 0} -> m:size_nat{m > 0} -> Tot (r:size_nat{r > 0 /\ x <= m * r})
 let blocks x m = (x - 1) / m + 1
 
-val xor_bytes: len:size_nat -> b1:lbytes len -> b2:lbytes len -> Tot (res:lbytes len)
-let xor_bytes len b1 b2 = map2 (fun x y -> logxor #U8 x y) b1 b2
+val xor_bytes: #len:size_nat -> b1:lbytes len -> b2:lbytes len -> Tot (res:lbytes len)
+let xor_bytes #len b1 b2 = map2 (fun x y -> logxor #U8 x y) b1 b2
 
-val eq_bytes: len:size_nat -> b1:lbytes len -> b2:lbytes len -> Tot bool
-let eq_bytes len b1 b2 = for_all2 (fun x y -> uint_to_nat #U8 x = uint_to_nat #U8 y) b1 b2
+val eq_bytes: #len:size_nat -> b1:lbytes len -> b2:lbytes len -> Tot bool
+let eq_bytes #len b1 b2 = for_all2 (fun x y -> uint_to_nat #U8 x = uint_to_nat #U8 y) b1 b2
 
 (* SHA256 *)
 let max_input_len_sha256 = pow2 61
 unfold let hLen = 32
+
 val hash_sha256:
-    msgLen:size_nat{msgLen < max_input_len_sha256} ->
-    msg:lbytes msgLen ->
-    hash:lbytes hLen ->
-    Tot (msgHash:lbytes hLen)
-let hash_sha256 msgLen msg hash = Hash.hash256 msgLen msg
+  #msgLen:size_nat{msgLen < max_input_len_sha256} ->
+  msg:lbytes msgLen -> Tot (msgHash:lbytes hLen)
+let hash_sha256 #msgLen msg = Hash.hash256 msgLen msg
 
 (* Mask Generation Function *)
-val mgf_sha256_loop:
-    mgfseedLen:size_nat{mgfseedLen = hLen + 4 /\ mgfseedLen < max_input_len_sha256} ->
-    mgfseed:lbytes mgfseedLen ->
-    counter_max:size_nat{counter_max * hLen < pow2 32}->
-    accLen:size_nat{accLen = counter_max * hLen} ->
-    acc:lbytes accLen ->
-    Tot (res:lbytes accLen)
-
-#reset-options "--z3rlimit 30 --max_fuel 0 --max_ifuel 0"
-
-let mgf_sha256_loop mgfseedLen mgfseed counter_max accLen acc =
-    let mHash = create hLen (u8 0) in
-    let next (i:size_nat{i < counter_max}) (acc:lbytes accLen) : lbytes accLen =
-        let counter = nat_to_bytes_be 4 i in
-        let mgfseed = update_sub mgfseed hLen 4 counter in
-        let mHash = hash_sha256 mgfseedLen mgfseed mHash in
-        update_sub acc (hLen * i) hLen mHash in
-    repeati #(lbytes accLen) counter_max next acc
-
-(* We only allow U32.t masklen, this means that we always have the property
-   that maskLen <= op_Multiply (pow2 32) (U32.v hLen) as required by the spec *)
+(* max_size_t = pow2 32 - 1 *)
 val mgf_sha256:
-    mgfseedLen:size_nat{mgfseedLen = hLen + 4 /\ mgfseedLen < max_input_len_sha256} ->
-    mgfseed:lbytes mgfseedLen ->
-    maskLen:size_nat{maskLen > 0 /\ (blocks maskLen hLen) * hLen < pow2 32} ->
-    mask:lbytes maskLen ->
-    Tot (mask':lbytes maskLen)
+  #mgfseedLen:size_nat{mgfseedLen + 4 < max_size_t /\ mgfseedLen + 4 < max_input_len_sha256} ->
+  mgfseed:lbytes mgfseedLen ->
+  maskLen:size_nat{0 < maskLen /\ (blocks maskLen hLen) * hLen < pow2 32} ->
+  Tot (mask:lbytes maskLen)
 
-#reset-options "--z3rlimit 50 --max_fuel 0"
+let mgf_sha256 #mgfseedLen mgfseed maskLen =
+  let counter_max = blocks maskLen hLen in
+  let accLen : size_nat = counter_max * hLen in
+  let acc = create accLen (u8 0) in
+  let mgfseed_counter = create (mgfseedLen + 4) (u8 0) in
+  let mgfseed_counter = update_slice mgfseed_counter 0 mgfseedLen mgfseed in
 
-let mgf_sha256 mgfseedLen mgfseed maskLen mask =
-    let counter_max = blocks maskLen hLen in
-    let accLen : size_nat = counter_max * hLen in
-    let acc = create accLen (u8 0) in
-    let acc = mgf_sha256_loop mgfseedLen mgfseed counter_max accLen acc in
-    slice acc 0 maskLen
+  let acc =
+    repeati counter_max
+    (fun i acc ->
+      let counter = nat_to_bytes_be 4 i in
+      let mgfseed_counter = update_slice mgfseed_counter mgfseedLen (mgfseedLen + 4) counter in
+      let mHash = hash_sha256 mgfseed_counter in
+      update_slice acc (hLen * i) (hLen * i + hLen) mHash
+    ) acc in
+  slice acc 0 maskLen
+
+(* Bignum convert functions *)
+val os2ip: #bLen:size_nat -> b:lbytes bLen -> Tot (res:nat{res < pow2 (8 * bLen)})
+let os2ip #bLen b = nat_from_intseq_be #U8 #bLen b
+
+val i2osp: #bLen:size_nat -> n:nat{n < pow2 (8 * bLen)} -> Tot (lbytes bLen)
+let i2osp #bLen n = nat_to_bytes_be bLen n
 
 (* RSA *)
-type modBits = modBits:size_nat{1 < modBits /\ modBits + 3 < pow2 32}
+type elem n = x:nat{x < n}
 
-noeq type rsa_pubkey (modBits:modBits) =
-     | Mk_rsa_pubkey: n:bignum{1 < n /\ pow2 (modBits - 1) <= n /\ n < pow2 modBits} ->
-                      e:elem n{1 < e} -> rsa_pubkey modBits
-	
-noeq type rsa_privkey (modBits:modBits) =
-     | Mk_rsa_privkey: pkey:rsa_pubkey modBits ->
-                       d:elem (Mk_rsa_pubkey?.n pkey){1 < d} ->
-                       p:elem (Mk_rsa_pubkey?.n pkey){1 < p} ->
-                       q:elem (Mk_rsa_pubkey?.n pkey){1 < q /\ (Mk_rsa_pubkey?.n pkey) = p * q} -> rsa_privkey modBits
+type modBits = modBits:size_nat{1 < modBits}
 
-val pss_encode_:
-    sLen:size_nat{sLen + hLen + 8 < pow2 32 /\ sLen + hLen + 8 < max_input_len_sha256} ->
-    salt:lbytes sLen ->
-    msgLen:size_nat{msgLen < max_input_len_sha256} ->
-    msg:lbytes msgLen ->
-    emLen:size_nat{0 <= emLen - sLen - hLen - 2 /\ emLen < pow2 32} ->
-    em:lbytes emLen ->
-    Tot (em':lbytes emLen)
+noeq type rsa_pubkey (x0:size_nat) (modBits:modBits) =
+  | Mk_rsa_pubkey: n:nat{1 < n /\ pow2 (modBits - 1) <= n /\ n < pow2 modBits /\ 2 * n < pow2 (pow2 x0)} ->
+                   e:elem n{1 < e} -> rsa_pubkey x0 modBits
 
-let pss_encode_ sLen salt msgLen msg emLen em =
-    let mHash = create hLen (u8 0) in
-    let mHash = hash_sha256 msgLen msg mHash in
-
-    //m1 = [8 * 0x00; mHash; salt]
-    let m1_size : size_nat = 8 + hLen + sLen in
-    let m1 = create m1_size (u8 0) in
-    let m1 = update_sub m1 8 hLen mHash in
-    let m1 = update_sub m1 (8 + hLen) sLen salt in
-    let m1Hash = create 36 (u8 0) in
-    let m1Hash' = sub m1Hash 0 hLen in
-    let m1Hash' = hash_sha256 m1_size m1 m1Hash' in
-    let m1Hash = update_sub m1Hash 0 hLen m1Hash' in
-
-    //db = [0x00; ..; 0x00; 0x01; salt]
-    let db_size : size_nat = emLen - hLen - 1 in
-    let db = create db_size (u8 0) in
-    let last_before_salt = db_size - sLen - 1 in
-    let db = db.[last_before_salt] <- (u8 1) in
-    let db = update_sub db (last_before_salt + 1) sLen salt in
-
-    let dbMask = create db_size (u8 0) in
-    let dbMask = mgf_sha256 (hLen + 4) m1Hash db_size dbMask in
-    let maskedDB = xor_bytes db_size db dbMask in
-    //em = [maskedDB; m1Hash'; 0xbc]
-    let em = update_sub em 0 db_size maskedDB in
-    let em = update_sub em db_size hLen m1Hash' in
-    em.[emLen - 1] <- (u8 0xbc)
+noeq type rsa_privkey (x0:size_nat) (modBits:modBits) =
+  | Mk_rsa_privkey: pkey:rsa_pubkey x0 modBits ->
+		    d:elem (Mk_rsa_pubkey?.n pkey){1 < d} ->
+		    p:elem (Mk_rsa_pubkey?.n pkey){1 < p} ->
+		    q:elem (Mk_rsa_pubkey?.n pkey){1 < q /\ (Mk_rsa_pubkey?.n pkey) = p * q} -> rsa_privkey x0 modBits
 
 val pss_encode:
-    msBits:size_nat{msBits < 8} ->
-    sLen:size_nat{sLen + hLen + 8 < pow2 32 /\ sLen + hLen + 8 < max_input_len_sha256} ->
-    salt:lbytes sLen ->
-    msgLen:size_nat{msgLen < max_input_len_sha256} ->
-    msg:lbytes msgLen ->
-    emLen:size_nat{0 <= emLen - sLen - hLen - 3 /\ emLen < pow2 32} ->
-    em:lbytes emLen ->
-    Tot (lbytes emLen)
+  #sLen:size_nat{sLen + hLen + 8 < max_size_t /\ sLen + hLen + 8 < max_input_len_sha256} ->
+  #msgLen:size_nat{msgLen < max_input_len_sha256} ->
+  salt:lbytes sLen ->
+  msg:lbytes msgLen ->
+  emBits:size_nat{emBits > 0 /\ hLen + sLen + 2 <= (blocks emBits 8)} -> Tot (lbytes (blocks emBits 8))
 
-let pss_encode msBits sLen salt msgLen msg emLen em =
-    if msBits = 0
-    then begin
-        let em' = sub em 1 (emLen - 1) in
-        let em' = pss_encode_ sLen salt msgLen msg (emLen - 1) em' in
-        update_sub em 1 (emLen - 1) em' end
-    else begin
-        let em = pss_encode_ sLen salt msgLen msg emLen em in
-        assert (0 < 8 - msBits /\ 8 - msBits < 8);
-        em.[0] <- logand #U8 em.[0] ((u8 0xff) >>. u32 (8 - msBits)) end
+let pss_encode #sLen #msgLen salt msg emBits =
+  let emLen = blocks emBits 8 in
+  let msBits = emBits % 8 in
 
-val pss_verify_:
-    sLen:size_nat{sLen + hLen + 8 < pow2 32 /\ sLen + hLen + 8 < max_input_len_sha256} ->
-    msBits:size_nat{msBits < 8} ->
-    emLen:size_nat{0 <= emLen - sLen - hLen - 2 /\ emLen < pow2 32} ->
-    em:lbytes emLen ->
-    msgLen:size_nat{msgLen < max_input_len_sha256} ->
-    msg:lbytes msgLen -> Tot bool
+  let mHash = hash_sha256 msg in
+  let m1Len:size_nat = 8 + hLen + sLen in
+  //m1 = [8 * 0x00; mHash; salt]
+  let m1 = create m1Len (u8 0) in
+  let m1 = update_slice m1 8 (8 + hLen) mHash in
+  let m1 = update_slice m1 (8 + hLen) m1Len salt in
+  let m1Hash = hash_sha256 #m1Len m1 in
 
-let pss_verify_ sLen msBits emLen em msgLen msg =
-    let mHash = create hLen (u8 0) in
-    let mHash = hash_sha256 msgLen msg mHash in
+  let dbLen:size_nat = emLen - hLen - 1 in
+  //db = [0x00;..; 0x00; 0x01; salt]
+  let db = create dbLen (u8 0) in
+  let last_before_salt = dbLen - sLen - 1 in
+  let db = db.[last_before_salt] <- (u8 1) in
+  let db = update_slice db (last_before_salt + 1) dbLen salt in
 
-    let (pad_size:size_nat{pad_size > 0}) = emLen - sLen - hLen - 1 in
-    let pad2 = create pad_size (u8 0) in
-    let pad2 = pad2.[pad_size - 1] <- (u8 0x01) in
+  let dbMask = mgf_sha256 m1Hash dbLen in
+  let maskedDB = xor_bytes db dbMask in
+  let maskedDB =
+    if msBits > 0 then
+      maskedDB.[0] <- logand #U8 maskedDB.[0] ((u8 0xff) >>. u32 (8 - msBits))
+    else maskedDB in
 
-    let (db_size:size_nat{db_size > 0}) = emLen - hLen - 1 in
-    let maskedDB = slice em 0 db_size in
-    let m1Hash0 = slice em db_size (db_size + hLen) in
-    let m1Hash = create 36 (u8 0) in
-    let m1Hash = update_sub m1Hash 0 hLen m1Hash0 in
-    let dbMask = create db_size (u8 0) in
-    let dbMask = mgf_sha256 (hLen + 4) m1Hash db_size dbMask in
-    let db = xor_bytes db_size maskedDB dbMask in
-    let db =
-        if msBits > 0
-        then begin
-            assert (0 < 8 - msBits /\ 8 - msBits < 8);
-            db.[0] <- logand #U8 db.[0] (u8 0xff >>. u32 (8 - msBits)) end
-        else db in
-	
-    let pad = slice db 0 pad_size in
-    let salt = slice db pad_size (pad_size + sLen) in
-
-    let m1_size:size_nat = 8 + hLen + sLen in
-    let m1 = create m1_size (u8 0) in
-    let m1Hash' = create hLen (u8 0) in
-    if not (eq_bytes pad_size pad pad2) then false
-    else begin
-        (* first 8 elements should be 0x00 *)
-        let m1 = update_sub m1 8 hLen mHash in
-        let m1 = update_sub m1 (8 + hLen) sLen salt in
-        let m1Hash' = hash_sha256 m1_size m1 m1Hash' in
-        eq_bytes hLen m1Hash0 m1Hash'
-    end
+  let em = create emLen (u8 0) in
+  //em = [maskedDB; m1Hash; 0xbc]
+  let em = update_slice em 0 dbLen maskedDB in
+  let em = update_slice em dbLen (dbLen + hLen) m1Hash in
+  em.[emLen - 1] <- (u8 0xbc)
 
 val pss_verify:
-    sLen:size_nat{sLen + hLen + 8 < pow2 32 /\ sLen + hLen + 8 < max_input_len_sha256} ->
-    msBits:size_nat{msBits < 8} ->
-    emLen:size_nat{0 < emLen /\ emLen < pow2 32} ->
-    em:lbytes emLen ->
-    msgLen:size_nat{msgLen < max_input_len_sha256} ->
-    msg:lbytes msgLen -> Tot bool
+  #msgLen:size_nat{msgLen < max_input_len_sha256} ->
+  sLen:size_nat{sLen + hLen + 8 < max_size_t /\ sLen + hLen + 8 < max_input_len_sha256} ->
+  msg:lbytes msgLen ->
+  emBits:size_nat{emBits > 0} ->
+  em:lbytes (blocks emBits 8) -> Tot bool
 
-let pss_verify sLen msBits emLen em msgLen msg =
-    let em_0 = em.[0] &. (u8 0xff <<. u32 msBits) in
-    let em_last = em.[emLen - 1] in
+let pss_verify #msgLen sLen msg emBits em =
+  let (emLen:size_nat{emLen > 0}) = blocks emBits 8 in
+  let msBits = emBits % 8 in
+  let mHash = hash_sha256 msg in
 
-    if not ((uint_to_nat #U8 em_0 = 0) && (uint_to_nat #U8 em_last = 0xbc))
-    then false
+  let em_0 = if msBits > 0 then em.[0] &. (u8 0xff <<. u32 msBits) else u8 0 in
+  let em_last = em.[emLen - 1] in
+
+  if (emLen < sLen + hLen + 2) then false
+  else begin
+    if (not (uint_to_nat #U8 em_last = 0xbc && uint_to_nat #U8 em_0 = 0)) then false
     else begin
-        let emLen' = if msBits = 0 then emLen - 1 else emLen in
-        let em':lbytes emLen' = if msBits = 0 then sub em 1 (emLen - 1) else em in
-        if (emLen' < sLen + hLen + 2)
-        then false
-        else pss_verify_ sLen msBits emLen' em' msgLen msg
+      let (dbLen:size_nat{dbLen > 0}) = emLen - hLen - 1 in
+      let maskedDB = slice em 0 dbLen in
+      let m1Hash = slice em dbLen (dbLen + hLen) in
+
+      let dbMask = mgf_sha256 m1Hash dbLen in
+      let db = xor_bytes maskedDB dbMask in
+      let db =
+	if msBits > 0
+	then db.[0] <- logand #U8 db.[0] (u8 0xff >>. u32 (8 - msBits))
+	else db in
+
+      let (padLen:size_nat{padLen > 0}) = emLen - sLen - hLen - 1 in
+      let pad2 = create padLen (u8 0) in
+      let pad2 = pad2.[padLen - 1] <- (u8 0x01) in
+
+      let pad = slice db 0 padLen in
+      let salt = slice db padLen (padLen + sLen) in
+
+      if not (eq_bytes pad pad2) then false
+      else begin
+	let m1Len:size_nat = 8 + hLen + sLen in
+	let m1 = create m1Len (u8 0) in
+	let m1 = update_slice m1 8 (8 + hLen) mHash in
+	let m1 = update_slice m1 (8 + hLen) m1Len salt in
+	let m1Hash0 = hash_sha256 #m1Len m1 in
+	eq_bytes m1Hash0 m1Hash
+      end
     end
+  end
 
-val rsa_sign:
-    x0:size_nat ->
-    modBits:modBits{pow2 (modBits + 2) < pow2 (pow2 x0)} ->
-    skey:rsa_privkey modBits ->
-    rBlind:bignum{rBlind < pow2 64} ->
-    sLen:size_nat{sLen + hLen + 8 < pow2 32 /\ 0 <= (blocks modBits 8) - sLen - hLen - 3 /\
-                  sLen + hLen + 8 < max_input_len_sha256} ->
-    salt:lbytes sLen ->
-    msgLen:size_nat{msgLen < max_input_len_sha256} ->
-    msg:lbytes msgLen ->
-    Tot (sgnt:lbytes (blocks modBits 8))
+val rsapss_sign:
+  #sLen:size_nat{sLen + hLen + 8 < max_size_t /\ sLen + hLen + 8 < max_input_len_sha256} ->
+  #msgLen:size_nat{msgLen < max_input_len_sha256} ->
+  x0:size_nat -> modBits:modBits{sLen + hLen + 2 <= (blocks (modBits - 1) 8)} ->
+  skey:rsa_privkey x0 modBits ->
+  salt:lbytes sLen -> rBlind:nat{rBlind < pow2 64} ->
+  msg:lbytes msgLen -> Tot (sgnt:lbytes (blocks modBits 8))
 
-let rsa_sign x0 modBits skey rBlind sLen salt msgLen msg =
-    let pkey = Mk_rsa_privkey?.pkey skey in
-    let n = Mk_rsa_pubkey?.n pkey in
-    let e = Mk_rsa_pubkey?.e pkey in
-    let d = Mk_rsa_privkey?.d skey in
-    let p = Mk_rsa_privkey?.p skey in
-    let q = Mk_rsa_privkey?.q skey in
-    let k = blocks modBits 8 in
-    assert (modBits <= 8 * k);
-    pow2_le_compat (8 * k) modBits;
-    assert (pow2 modBits <= pow2 (8 * k));
-    assert (n < pow2 (8 * k));
-	
-    let msBits = (modBits - 1) % 8 in
-    let em = create k (u8 0) in
-    let em = pss_encode msBits sLen salt msgLen msg k em in
-    let m = os2ip k em in
-	
-    assume (m < n);
-    let s = rsa_blinding x0 modBits n p q d m rBlind in
+let rsapss_sign #sLen #msgLen x0 modBits skey salt rBlind msg =
+  let pkey = Mk_rsa_privkey?.pkey skey in
+  let n = Mk_rsa_pubkey?.n pkey in
+  let e = Mk_rsa_pubkey?.e pkey in
+  let d = Mk_rsa_privkey?.d skey in
+  let p = Mk_rsa_privkey?.p skey in
+  let q = Mk_rsa_privkey?.q skey in
 
-    let sgnt = create k (u8 0) in
-    assert (s < n);
-    i2osp s k sgnt
+  let nLen = blocks modBits 8 in
+  assert (modBits <= 8 * nLen);
+  pow2_le_compat (8 * nLen) modBits;
+  assert (pow2 modBits <= pow2 (8 * nLen));
+  assert (n < pow2 (8 * nLen));
 
-val rsa_verify:
-    x0:size_nat ->
-    modBits:modBits{pow2 (modBits + 2) < pow2 (pow2 x0)} ->
-    pkey:rsa_pubkey modBits ->
-    sLen:size_nat{sLen + hLen + 8 < pow2 32 /\ sLen + hLen + 8 < max_input_len_sha256} ->
-    sgnt:lbytes (blocks modBits 8) ->
-    msgLen:size_nat{msgLen < max_input_len_sha256} ->
-    msg:lbytes msgLen -> Tot bool
+  let emBits = modBits - 1 in
+  let em = pss_encode #sLen #msgLen salt msg emBits in
+  let emLen = blocks emBits 8 in
+  let m = os2ip #emLen em in
+  assume (m < n);
 
-let rsa_verify x0 modBits pkey sLen sgnt msgLen msg =
-    let n = Mk_rsa_pubkey?.n pkey in
-    let e = Mk_rsa_pubkey?.e pkey in
-    let k = blocks modBits 8 in
-    assert (modBits <= 8 * k);
-    pow2_le_compat (8 * k) modBits;
-    assert (pow2 modBits <= pow2 (8 * k));
-    assert (n < pow2 (8 * k));
+  let s = rsa_blinding x0 modBits n p q d m rBlind in
+  assert (s < n);
+  i2osp #nLen s
 
-    let s = os2ip k sgnt in
-    if bn_is_less s n then begin
-        assert (s < n);
-        let m = mod_exp x0 modBits n s e in
-        let em = create k (u8 0) in
-        let em = i2osp m k em in
-        let msBits = (modBits - 1) % 8 in
-        pss_verify sLen msBits k em msgLen msg end
-    else false
+val rsapss_verify:
+  #msgLen:size_nat{msgLen < max_input_len_sha256} ->
+  x0:size_nat -> modBits:modBits ->
+  pkey:rsa_pubkey x0 modBits ->
+  sLen:size_nat{sLen + hLen + 8 < max_size_t /\ sLen + hLen + 8 < max_input_len_sha256} ->
+  msg:lbytes msgLen ->
+  sgnt:lbytes (blocks modBits 8) -> Tot bool
+
+let rsapss_verify #msgLen x0 modBits pkey sLen msg sgnt =
+  let n = Mk_rsa_pubkey?.n pkey in
+  let e = Mk_rsa_pubkey?.e pkey in
+  let nLen = blocks modBits 8 in
+  assert (modBits <= 8 * nLen);
+  pow2_le_compat (8 * nLen) modBits;
+  assert (pow2 modBits <= pow2 (8 * nLen));
+  assert (n < pow2 (8 * nLen));
+
+  let s = os2ip #nLen sgnt in
+  if s < n then begin
+    let m = mod_exp x0 modBits n s e in
+    let emBits = modBits - 1 in
+    let emLen = blocks emBits 8 in
+    assume (m < pow2 (emLen * 8));
+    let em = i2osp #emLen m in
+    pss_verify #msgLen sLen msg emBits em end
+  else false
